Rename inv_46_b_ii to inv_46_b

src/dvspec/dafny/att_spec_proofs/inv.dfy
@@ -2132,29 +2132,7 @@ module Att_Inv_With_Empty_Initial_Attestation_Slashing_DB
                     ==> s in hn_state.attestation_consensus_engine_state.att_slashing_db_hist.Keys)
     }
 
-    predicate inv46_b_body(dvn: DVState, hn: BLSPubkey, s: Slot, vp: AttestationData -> bool)
-    requires hn in dvn.honest_nodes_states.Keys
-    requires hn in dvn.consensus_on_attestation_data[s].honest_nodes_validity_functions.Keys
-    requires s in dvn.honest_nodes_states[hn].attestation_consensus_engine_state.att_slashing_db_hist.Keys
-    {
-        && var hn_state := dvn.honest_nodes_states[hn];
-        && ( vp in dvn.consensus_on_attestation_data[s].honest_nodes_validity_functions[hn]
-                ==> vp in hn_state.attestation_consensus_engine_state.att_slashing_db_hist[s] )
-    }
-    
-    predicate inv46_b(dvn: DVState)
-    {
-        forall hn: BLSPubkey, s: Slot ::
-            && is_honest_node(dvn, hn) 
-            && var hn_state := dvn.honest_nodes_states[hn];
-            && hn in dvn.consensus_on_attestation_data[s].honest_nodes_validity_functions.Keys
-            && s in hn_state.attestation_consensus_engine_state.att_slashing_db_hist.Keys
-            ==> ( forall vp: AttestationData -> bool ::
-                    inv46_b_body(dvn, hn, s, vp)
-                )                    
-    }  
-
-    predicate inv46_b_ii_body(
+    predicate inv46_b_body(
         dvn: DVState, 
         hn: BLSPubkey,
         hn_state: DVCNodeState,
@@ -2176,12 +2154,12 @@ module Att_Inv_With_Empty_Initial_Attestation_Slashing_DB
         )             
     }       
     
-    predicate inv46_b_ii(dvn: DVState)
+    predicate inv46_b(dvn: DVState)
     {
         forall hn: BLSPubkey, s: Slot, vp : AttestationData -> bool |
             hn in dvn.honest_nodes_states.Keys
             ::
-            inv46_b_ii_body(
+            inv46_b_body(
                 dvn,
                 hn,
                 dvn.honest_nodes_states[hn],
